Rework recover spec and nearly prove top-level theorem
I changed the statement of recover_ok to split out the two cases and
make sure the variable for the current memory is only created if
necessary. This allowed me to prove simple corr3 relations in
ExampleMemLog, and very nearly works for write_block_inbounds
too, except that I ran into a problem with fsxp that I can't quite
solve (and I'm worried something similar will show up trying to
prove recover_ok).

I also renamed "would_recover_either" to "log_intact" and
"might_recover_cur" to "would_recover_either".

src/FS.v
@@ -106,26 +106,18 @@ Theorem read_block_ok : forall fsxp inum off mscs,
   POST:(mscs',r)
          MEMLOG.rep (FSXPMemLog fsxp) (NoTransaction m) mscs' *
          [[ r = v ]]
-  CRASH  MEMLOG.log_intact (FSXPMemLog fsxp) m
+  CRASH  MEMLOG.log_intact (FSXPMemLog fsxp) m m
   >} read_block fsxp inum off mscs.
 Proof.
-(* XXX why doesn't this proof, which unfolds MEM.log_intact first, go through?
-  unfold read_block, MEMLOG.log_intact.
-  hoare.
-  admit.
-  unfold MEMLOG.log_intact; cancel.
-*)
-
   unfold read_block.
-  hoare.
-  admit.
-  unfold MEMLOG.log_intact; cancel.
-  unfold MEMLOG.log_intact; cancel.
+  hoare_unfold MEMLOG.log_intact_unfold.
 Qed.
+
 
 Theorem read_block_recover_ok : forall fsxp inum off mscs cachesize,
   {< m F flist A f B v,
-  PRE     MEMLOG.rep (FSXPMemLog fsxp) (NoTransaction m) mscs *
+  PRE     [[ cachesize <> 0 ]] *
+          MEMLOG.rep (FSXPMemLog fsxp) (NoTransaction m) mscs *
           [[ (F * BFILE.rep (FSXPBlockAlloc fsxp) (FSXPInode fsxp) flist)%pred (list2mem m) ]] *
           [[ (A * #inum |-> f)%pred (list2nmem flist) ]] *
           [[ (B * #off |-> v)%pred (list2nmem (BFILE.BFData f)) ]]
@@ -137,7 +129,7 @@ Theorem read_block_recover_ok : forall fsxp inum off mscs cachesize,
 Proof.
   intros.
   unfold forall_helper; intros m F flist A f B v.
-  exists (MEMLOG.log_intact (FSXPMemLog fsxp) m).
+  exists (MEMLOG.log_intact (FSXPMemLog fsxp) m m).
 
   intros.
   eapply pimpl_ok3.
@@ -149,12 +141,25 @@ Proof.
   step.
   cancel.
   cancel.
-  rewrite crash_xform_sep_star_dist.
-  instantiate (a:=m). instantiate (a0:=m).
-  admit.
+  unfold MEMLOG.log_intact.
+  autorewrite with crash_xform.
+  rewrite sep_star_or_distr.
+  apply pimpl_or_l.
+  cancel.
+  autorewrite with crash_xform.
+  rewrite sep_star_comm.
+  apply pimpl_or_r; left; cancel.
 
+  unfold MEMLOG.log_intact in *.
   step.
-  admit.
+  rewrite H3; cancel.
+  cancel.
+
+  unfold MEMLOG.log_intact in *.
+  apply pimpl_or_r; right; cancel.
+  step.
+  rewrite H3; cancel.
+  cancel.
 Qed.
 
 Definition write_block_inbounds T fsxp inum off v mscs rx : prog T :=
@@ -176,45 +181,54 @@ Theorem write_block_inbounds_ok : forall fsxp inum off v mscs,
           [[ (F * BFILE.rep (FSXPBlockAlloc fsxp) (FSXPInode fsxp) flist')%pred (list2mem m') ]] *
           [[ (A * #inum |-> f')%pred (list2nmem flist') ]] *
           [[ (B * #off |-> v)%pred (list2nmem (BFILE.BFData f')) ]]
-  CRASH   MEMLOG.log_intact (FSXPMemLog fsxp) m \/ exists m' flist' f',
-          MEMLOG.log_intact (FSXPMemLog fsxp) m' *
+  CRASH   MEMLOG.would_recover_old (FSXPMemLog fsxp) m \/ exists m' flist' f',
+          MEMLOG.would_recover_either (FSXPMemLog fsxp) m m' *
           [[ (F * BFILE.rep (FSXPBlockAlloc fsxp) (FSXPInode fsxp) flist')%pred (list2mem m') ]] *
           [[ (A * #inum |-> f')%pred (list2nmem flist') ]] *
           [[ (B * #off |-> v)%pred (list2nmem (BFILE.BFData f')) ]]
   >} write_block_inbounds fsxp inum off v mscs.
 Proof.
   unfold write_block_inbounds.
-  hoare.
-  admit.
-  unfold MEMLOG.log_intact; cancel.
-  unfold MEMLOG.log_intact; cancel.
+  hoare_unfold MEMLOG.log_intact_unfold.
 Qed.
 
+Definition write_block_inbounds' fsxp inum off v T := @write_block_inbounds T fsxp inum off v.
+
 Theorem write_block_inbounds_recover_ok : forall fsxp inum off v mscs cachesize,
-  {< m F flist A f B v0,
-  PRE     MEMLOG.rep (FSXPMemLog fsxp) (NoTransaction m) mscs *
-          [[ (F * BFILE.rep (FSXPBlockAlloc fsxp) (FSXPInode fsxp) flist)%pred (list2mem m) ]] *
-          [[ (A * #inum |-> f)%pred (list2nmem flist) ]] *
-          [[ (B * #off |-> v0)%pred (list2nmem (BFILE.BFData f)) ]]
+  {< flist A f B v0 F m,
+  PRE     [[ cachesize <> 0 ]] *
+          MEMLOG.rep (FSXPMemLog fsxp) (NoTransaction m) mscs *
+          [[ (F * BFILE.rep (FSXPBlockAlloc fsxp) (FSXPInode fsxp) flist *
+            [[ (A * #inum |-> f)%pred (list2nmem flist) ]] *
+            [[ (B * #off |-> v0)%pred (list2nmem (BFILE.BFData f)) ]])%pred (list2mem m) ]]
   POST:(mscs',ok)
           [[ ok = false ]] * MEMLOG.rep (FSXPMemLog fsxp) (NoTransaction m) mscs' \/
-          [[ ok = true ]] * exists m' flist' f',
+          [[ ok = true ]] * exists m',
           MEMLOG.rep (FSXPMemLog fsxp) (NoTransaction m') mscs' *
-          [[ (F * BFILE.rep (FSXPBlockAlloc fsxp) (FSXPInode fsxp) flist')%pred (list2mem m') ]] *
-          [[ (A * #inum |-> f')%pred (list2nmem flist') ]] *
-          [[ (B * #off |-> v)%pred (list2nmem (BFILE.BFData f')) ]]
+          [[ (exists flist' f', F * BFILE.rep (FSXPBlockAlloc fsxp) (FSXPInode fsxp) flist' *
+            [[ (A * #inum |-> f')%pred (list2nmem flist') ]] *
+            [[ (B * #off |-> v)%pred (list2nmem (BFILE.BFData f')) ]])%pred (list2mem m') ]]
   CRASH:r
-          MEMLOG.rep (FSXPMemLog (snd r)) (NoTransaction m) (fst r) \/ exists m' flist' f',
+          MEMLOG.rep (FSXPMemLog (snd r)) (NoTransaction m) (fst r) \/ exists m',
           MEMLOG.rep (FSXPMemLog (snd r)) (NoTransaction m') (fst r) *
-          [[ (F * BFILE.rep (FSXPBlockAlloc (snd r)) (FSXPInode (snd r)) flist')%pred (list2mem m') ]] *
-          [[ (A * #inum |-> f')%pred (list2nmem flist') ]] *
-          [[ (B * #off |-> v)%pred (list2nmem (BFILE.BFData f')) ]]
+          [[ (exists flist' f', F * BFILE.rep (FSXPBlockAlloc (snd r)) (FSXPInode (snd r)) flist' *
+            [[ (A * #inum |-> f')%pred (list2nmem flist') ]] *
+            [[ (B * #off |-> v)%pred (list2nmem (BFILE.BFData f')) ]])%pred (list2mem m') ]]
   >} write_block_inbounds fsxp inum off v mscs >> MEMLOG.recover cachesize.
 Proof.
   intros.
-  unfold forall_helper; intros m F flist A f B v0.
-  exists (MEMLOG.log_intact (FSXPMemLog fsxp) m \/ exists m' flist' f',
-          MEMLOG.log_intact (FSXPMemLog fsxp) m' *
+  (*unfold forall_helper at 1 2 3 4 5; intros flist A f B v0 F.
+  Check (MEMLOG.recover_corr2_to_corr3 (write_block_inbounds' fsxp inum off v)
+    (F * BFILE.rep (FSXPBlockAlloc fsxp) (FSXPInode fsxp) flist *
+            [[ (A * #inum |-> f)%pred (list2nmem flist) ]] *
+            [[ (B * #off |-> v0)%pred (list2nmem (BFILE.BFData f)) ]] )
+    (exists flist' f', F * BFILE.rep (FSXPBlockAlloc fsxp) (FSXPInode fsxp) flist' *
+            [[ (A * #inum |-> f')%pred (list2nmem flist') ]] *
+            [[ (B * #off |-> v)%pred (list2nmem (BFILE.BFData f')) ]])%pred).*)
+
+  unfold forall_helper; intros flist A f B v0 F m.
+  exists (MEMLOG.would_recover_old (FSXPMemLog fsxp) m \/ exists m' flist' f',
+          MEMLOG.would_recover_either (FSXPMemLog fsxp) m m' *
           [[ (F * BFILE.rep (FSXPBlockAlloc fsxp) (FSXPInode fsxp) flist')%pred (list2mem m') ]] *
           [[ (A * #inum |-> f')%pred (list2nmem flist') ]] *
           [[ (B * #off |-> v)%pred (list2nmem (BFILE.BFData f')) ]])%pred.
@@ -229,39 +243,53 @@ Proof.
   step.
   cancel.
   cancel.
-
+  auto.
+  unfold MEMLOG.log_intact.
+  autorewrite with crash_xform.
+  rewrite sep_star_or_distr.
+  apply pimpl_or_l.
   cancel.
-  cancel.
-  cancel.
-
-  rewrite crash_xform_sep_star_dist.
-  rewrite crash_xform_or_dist.
-  cancel.
-  admit.
-  step.
-
-  instantiate (p:=p). instantiate (a:=m). cancel.
-  apply pimpl_or_r; left. cancel.
-
-  instantiate (a0:=m). cancel.
-
-  apply pimpl_or_r; left. cancel.
-
-  cancel. apply pimpl_or_r; left.
-  admit.
-
-  admit.
+  autorewrite with crash_xform.
+  apply pimpl_or_r; left; cancel.
 
   step.
+  rewrite sep_star_or_distr.
+  apply pimpl_or_r; left; cancel.
+  rewrite H3; auto.
+  rewrite H3; cancel.
+  apply pimpl_or_r; left; cancel.
 
-  instantiate (p:=p).
-  instantiate (a2:=m). cancel.
-  apply pimpl_or_r; left. cancel.
-
-  instantiate (a3:=m). cancel.
-  apply pimpl_or_r; left. cancel.
-
+  rewrite H3.
+  autorewrite with crash_xform.
+  norm'l; unfold stars; simpl.
+  autorewrite with crash_xform.
+  norm'l; unfold stars; simpl.
+  autorewrite with crash_xform.
+  norm'l; unfold stars; simpl.
+  autorewrite with crash_xform.
   cancel.
+  apply pimpl_or_r; right.
+  norm.
+  (* XXX do this without the instantiate *)
+  instantiate (p := (p * [[(F * BFILE.rep (FSXPBlockAlloc fsxp) (FSXPInode fsxp) l)%pred (list2mem d)]] *
+    [[(A * # (inum) |-> b)%pred (list2nmem l)]] * [[(B * # (off) |-> v)%pred (list2nmem (BFILE.BFData b))]])%pred).
+  cancel.
+  intuition.
+
+  eapply pimpl_ok2; [ eauto |].
+  intros; norm.
+  unfold stars; simpl.
+  cancel.
+  cancel.
+  intuition.
+  subst.
+  auto.
+  unfold stars; simpl.
+  cancel.
+  apply pimpl_or_r; right.
+  (* XXX don't know that fsxp = b0 *)
+  admit.
+  admit.
   admit.
 Qed.
 
@@ -304,14 +332,14 @@ Theorem set_size_helper_ok : forall fsxp inum size mscs,
              [[ (F * BFILE.rep (FSXPBlockAlloc fsxp) (FSXPInode fsxp) flist)%pred (list2mem m) ]] *
              [[ (A * #inum |-> f)%pred (list2nmem flist) ]]
     POST:(mscs',r)
-             [[ r = false ]] * MEMLOG.log_intact (FSXPMemLog fsxp) mbase \/
+             [[ r = false ]] * MEMLOG.would_recover_old (FSXPMemLog fsxp) mbase \/
              [[ r = true ]] * exists m' flist' f',
              MEMLOG.rep (FSXPMemLog fsxp) (ActiveTxn mbase m') mscs' *
              [[ (F * BFILE.rep (FSXPBlockAlloc fsxp) (FSXPInode fsxp) flist')%pred (list2mem m') ]] *
              [[ (A * #inum |-> f')%pred (list2nmem flist') ]] *
              [[ BFILE.BFData f' = (firstn #size (BFILE.BFData f)) ++
                                   (repeat $0 (#size - length (BFILE.BFData f))) ]]
-    CRASH    MEMLOG.log_intact (FSXPMemLog fsxp) mbase
+    CRASH    MEMLOG.would_recover_old (FSXPMemLog fsxp) mbase
     >} set_size_helper fsxp inum size mscs.
 Proof.
   admit.
