src/Balloc.v
@@ -125,10 +125,10 @@ Module BALLOC.
                [[ (bn < BmapNBlocks xp ^* $ valulen)%word ]]
     POST:mscs' exists m', MEMLOG.rep lxp (ActiveTxn mbase m') mscs' *
                [[ (Fm * rep' xp (fupd bmap bn Avail))%pred (list2mem m') ]]
-    CRASH      MEMLOG.log_intact lxp mbase
+    CRASH      MEMLOG.would_recover_old lxp mbase
     >} free' lxp xp bn mscs.
   Proof.
-    unfold free', rep', valid_block, MEMLOG.log_intact.
+    unfold free', rep', valid_block, MEMLOG.would_recover_old.
     hoare.
     erewrite upd_bmap_bits; try trivial.
     cancel.
@@ -146,7 +146,7 @@ Module BALLOC.
       Invariant
         MEMLOG.rep lxp (ActiveTxn mbase m) mscs
       OnCrash
-        MEMLOG.log_intact lxp mbase
+        MEMLOG.would_recover_old lxp mbase
       Begin
         let2 (mscs, bit) <- RecArray.get itemtype items_per_valu blocksz
           lxp (xp_to_raxp xp) i mscs;
@@ -173,7 +173,7 @@ Module BALLOC.
                    MEMLOG.rep lxp (ActiveTxn mbase m') mscs' *
                    [[ (Fm * rep' xp (fupd bmap bn InUse))%pred (list2mem m') ]] *
                    [[ valid_block xp bn ]]
-    CRASH          MEMLOG.log_intact lxp mbase
+    CRASH          MEMLOG.would_recover_old lxp mbase
     >} alloc' lxp xp mscs.
   Proof.
     unfold alloc', rep'.
@@ -205,7 +205,7 @@ Module BALLOC.
                 (RecArray.Build_xparams (BmapStart xp) i)
                 (map (fun _ => $0) (seq 0 (#i * valulen))))%pred (list2mem m') ]]
       OnCrash
-        MEMLOG.log_intact lxp mbase
+        MEMLOG.would_recover_old lxp mbase
       Begin
         mscs <- MEMLOG.write_array lxp (BmapStart xp) i $1 $0 mscs;
         lrx mscs
@@ -223,7 +223,7 @@ Module BALLOC.
                 [[ goodSize addrlen (# (BmapNBlocks xp) * valulen) ]]
     POST:mscs'  exists m', MEMLOG.rep lxp (ActiveTxn mbase m') mscs' *
                 [[ (F * rep' xp bmap0)%pred (list2mem m') ]]
-    CRASH       MEMLOG.log_intact lxp mbase
+    CRASH       MEMLOG.would_recover_old lxp mbase
     >} init' lxp xp mscs.
   Proof.
     unfold init', rep'.
@@ -245,7 +245,7 @@ Module BALLOC.
     erewrite wordToNat_natToWord_bound with (bound:=BmapNBlocks xp); omega.
 
     admit.
-    unfold MEMLOG.log_intact; cancel.
+    unfold MEMLOG.would_recover_old; cancel.
     step.
     admit.
   Qed.
@@ -277,7 +277,7 @@ Module BALLOC.
                    [[ genpred =p=> genpred' * bn |->? ]] *
                    [[ genpredn =p=> genpredn' * #bn |->? ]] *
                    [[ valid_block xp bn ]]
-    CRASH          MEMLOG.log_intact lxp mbase
+    CRASH          MEMLOG.would_recover_old lxp mbase
     >} alloc_gen lxp xp mscs.
   Proof.
     unfold alloc_gen.
@@ -323,7 +323,7 @@ Module BALLOC.
                [[ (Fm * @rep_gen V xp (bn :: freeblocks) genpred' genpredn')%pred (list2mem m') ]] *
                [[ bn |->? * genpred =p=> genpred' ]] *
                [[ #bn |->? * genpredn =p=> genpredn' ]]
-    CRASH      MEMLOG.log_intact lxp mbase
+    CRASH      MEMLOG.would_recover_old lxp mbase
     >} free_gen lxp xp bn mscs.
   Proof.
     unfold free_gen.
@@ -361,7 +361,7 @@ Module BALLOC.
                    MEMLOG.rep lxp (ActiveTxn mbase m') mscs' *
                    [[ (Fm * bn |->? * rep xp freeblocks')%pred (list2mem m') ]] *
                    [[ valid_block xp bn ]]
-    CRASH          MEMLOG.log_intact lxp mbase
+    CRASH          MEMLOG.would_recover_old lxp mbase
     >} alloc lxp xp mscs.
   Proof.
     unfold alloc, rep.
@@ -381,7 +381,7 @@ Module BALLOC.
                [[ (bn < BmapNBlocks xp ^* $ valulen)%word ]]
     POST:mscs' exists m', MEMLOG.rep lxp (ActiveTxn mbase m') mscs' *
                [[ (Fm * rep xp (bn :: freeblocks))%pred (list2mem m') ]]
-    CRASH      MEMLOG.log_intact lxp mbase
+    CRASH      MEMLOG.would_recover_old lxp mbase
     >} free lxp xp bn mscs.
   Proof.
     unfold free, rep.
